code/ecdsap256/Hacl.Impl.P256.LowLevel.PrimeSpecific.fsti
@@ -18,6 +18,19 @@ let prime256_buffer: x: glbuffer uint64 4ul {witnessed #uint64 #(size 4) x (Lib.
   assert_norm (felem_seq_as_nat P256 (Lib.Sequence.of_list (p256_prime_list)) == prime256);
   createL_global p256_prime_list
 
+
+inline_for_extraction
+let prime384_buffer: x: glbuffer uint64 6ul {witnessed #uint64 #(size 6) x (Lib.Sequence.of_list
+p384_prime_list) /\ recallable x /\ felem_seq_as_nat P384 (Lib.Sequence.of_list (p384_prime_list)) == prime384}  = 
+  assert_norm (felem_seq_as_nat P384 (Lib.Sequence.of_list (p384_prime_list)) == prime384);
+  createL_global p384_prime_list
+
+
+inline_for_extraction
+let prime_buffer (#c: curve) (x: glbuffer uint64 (getCoordinateLenU64 c) {witnessed #uint64 #(getCoordinateLenU64 c) x (Lib.Sequence.of_list (prime_list c)) /\ recallable x /\ felem_seq_as_nat c (Lib.Sequence.of_list (prime_list c)) == getPrime c}) = 
+  createL_global (prime_list c)
+
+
 val reduction_prime_2prime_with_carry: #c: curve -> x: widefelem c -> result: felem c -> 
   Stack unit 
     (requires fun h -> 
