code/ecdsap256/Hacl.Spec.P256.Definition.fst
@@ -32,6 +32,55 @@ let p256_prime_list : x:list uint64{List.Tot.length x == 4 /\
 
 
 inline_for_extraction noextract
+let p384_prime_list : x:list uint64{List.Tot.length x == 6 /\ 
+  (
+    let open FStar.Mul in 
+    let l0 = uint_v (List.Tot.index x 0) in 
+    let l1 = uint_v (List.Tot.index x 1) in 
+    let l2 = uint_v (List.Tot.index x 2) in 
+    let l3 = uint_v (List.Tot.index x 3) in 
+    let l4 = uint_v (List.Tot.index x 4) in 
+    let l5 = uint_v (List.Tot.index x 5) in 
+    l0 + l1 * pow2 64 + l2 * pow2 128 + l3 * pow2 192 + l4 * pow2 256 + l5 * pow2 320 == prime384)
+  } =
+  let open FStar.Mul in 
+  [@inline_let]
+  let x =
+    [ (u64 0xffffffffffffffff);  (u64 0xffffffff); (u64 0);  (u64 0xffffffff00000001);] in
+    assert_norm(0xffffffff + 0xffffffff00000000 * pow2 64 + 0xfffffffffffffffe * pow2 128 + 
+    0xffffffffffffffff * pow2 192 +  0xffffffffffffffff * pow2 256 +  0xffffffffffffffff * pow2 320 == prime384);
+  x
+
+
+inline_for_extraction noextract
+let prime_list (c: curve) :  (x: list uint64 {List.Tot.length x == uint_v (getCoordinateLenU64 c) /\ (
+  match c with
+  |P256 -> 
+    let open FStar.Mul in 
+    let l0 = uint_v (List.Tot.index x 0) in 
+    let l1 = uint_v (List.Tot.index x 1) in 
+    let l2 = uint_v (List.Tot.index x 2) in 
+    let l3 = uint_v (List.Tot.index x 3) in 
+    l0 + l1 * pow2 64 + l2 * pow2 128 + l3 * pow2 192 == prime256
+  |P384 -> 
+    let open FStar.Mul in 
+    let l0 = uint_v (List.Tot.index x 0) in 
+    let l1 = uint_v (List.Tot.index x 1) in 
+    let l2 = uint_v (List.Tot.index x 2) in 
+    let l3 = uint_v (List.Tot.index x 3) in 
+    let l4 = uint_v (List.Tot.index x 4) in 
+    let l5 = uint_v (List.Tot.index x 5) in 
+    l0 + l1 * pow2 64 + l2 * pow2 128 + l3 * pow2 192 + l4 * pow2 256 + l5 * pow2 320 == prime384
+)}) = 
+  let open FStar.Mul in 
+  match c with 
+  |P256 -> 
+    p256_prime_list
+  |P384 -> 
+    p384_prime_list
+
+
+inline_for_extraction noextract
 let felem_coordinate (c: curve) =
   match c with 
   |P256 -> tuple4 uint64 uint64 uint64 uint64
